src/typechecker/FStarC.TypeChecker.Core.fsti
@@ -14,16 +14,16 @@
    limitations under the License.
 *)
 module FStarC.TypeChecker.Core
-#push-options "--MLish --MLish_effect FStarC.Effect"
 
 open FStarC
+open FStarC.Effect
 open FStarC.Syntax.Syntax
 open FStarC.TypeChecker.Common
 open FStarC.Class.Show
 module Env = FStarC.TypeChecker.Env
 
 
-type guard_commit_token_cb = unit -> unit
+type guard_commit_token_cb = unit -> ML unit
 (* The guard t is a precondition of typing computed by the core checker;
    Once the guard is proven, the caller should call commit_guard on the 
    guard_commit_token_cb to notify the core checker that the guard was
@@ -34,56 +34,59 @@ type tot_or_ghost =
   | E_Total
   | E_Ghost
 
-instance val showable_tot_or_ghost : Class.Show.showable tot_or_ghost
-
-val clear_memo_table (_:unit)
-  : unit
-
-val error : Type0
-instance val showable_error : showable error
-
 type side = 
   | Left
   | Right
   | Both
   | Neither
 
-instance val showable_side : Class.Show.showable side
+(* val declarations ordered to match .fst definition order *)
+
+val get_goal_ctr (_:unit) : ML int
+val incr_goal_ctr (_:unit) : ML int
+
+val error : Type0
+
+val print_error (err:error)
+  : ML string
+
+instance val showable_error : showable error
+
+val print_error_short (err:error)
+  : ML string
+
+val clear_memo_table (_:unit)
+  : ML unit
 
 val empty_token : guard_commit_token_cb
-val commit_guard (tok:guard_commit_token_cb) : unit
-val commit_guard_and_tok_opt (_: option guard_and_tok_t) : unit
-val maybe_relate_after_unfolding (g:Env.env) (t0 t1:term) : side
+val commit_guard (tok:guard_commit_token_cb) : ML unit
+val commit_guard_and_tok_opt (_: option guard_and_tok_t) : ML unit
 
-val is_non_informative (g:Env.env) (t:typ) : bool
+val is_non_informative (g:Env.env) (t:typ) : ML bool
+
+instance val showable_tot_or_ghost : Class.Show.showable tot_or_ghost
+instance val showable_side : Class.Show.showable side
+
+val maybe_relate_after_unfolding (g:Env.env) (t0 t1:term) : ML side
 
 val check_term (g:Env.env) (e:term) (t:typ) (must_tot:bool)
-  : either (option guard_and_tok_t) error
+  : ML (either (option guard_and_tok_t) error)
 
 val check_term_at_type (g:Env.env) (e:term) (t:typ)
-  : either (tot_or_ghost & option guard_and_tok_t) error
+  : ML (either (tot_or_ghost & option guard_and_tok_t) error)
 
 val compute_term_type (g:Env.env) (e:term)
-  : either (tot_or_ghost & typ & option guard_and_tok_t) error
+  : ML (either (tot_or_ghost & typ & option guard_and_tok_t) error)
 
 val open_binders_in_term (g:Env.env) (bs:binders) (t:term)
-  : Env.env & binders & term
+  : ML (Env.env & binders & term)
 
 val open_binders_in_comp (g:Env.env) (bs:binders) (c:comp)
-  : Env.env & binders & comp
+  : ML (Env.env & binders & comp)
 
 (* For unit testing, and exposed to tactics *)
 val check_term_equality (guard_ok:bool) (unfolding_ok:bool) (g:Env.env) (t0 t1:typ)
-  : either (option guard_and_tok_t) error
+  : ML (either (option guard_and_tok_t) error)
 
 val check_term_subtyping (guard_ok:bool) (unfolding_ok:bool) (g:Env.env) (t0 t1:typ)
-  : either (option guard_and_tok_t) error
-
-val print_error (err:error)
-  : string
-
-val print_error_short (err:error)
-  : string
-
-val get_goal_ctr (_:unit) : int
-val incr_goal_ctr (_:unit) : int
+  : ML (either (option guard_and_tok_t) error)
