src/syntax/FStarC.Syntax.DsEnv.fsti
@@ -15,8 +15,6 @@
 *)
 
 module FStarC.Syntax.DsEnv
-#push-options "--MLish --MLish_effect FStarC.Effect"
-
 open FStarC
 open FStarC.Effect
 open FStarC.Syntax
@@ -41,8 +39,15 @@ type record_or_dc = {
 
 val env : Type0
 val dsenv_hooks : Type0
-val parsing_data_for_scope (e:env) : list FStarC.Parser.Dep.parsing_data_elt
-val with_restored_scope (e:env) (f: env -> 'a & env) : 'a & env
+
+type withenv 'a = env -> 'a & env
+
+type foundname =
+  | Term_name of typ & list attribute
+  | Eff_name  of sigelt & lident
+
+val parsing_data_for_scope (e:env) : ML (list FStarC.Parser.Dep.parsing_data_elt)
+val with_restored_scope (e:env) (f: env -> 'a & env) : ML ('a & env)
 
 instance val showable_env : showable env
 val mk_dsenv_hooks
@@ -51,99 +56,86 @@ val mk_dsenv_hooks
   (module_abbrev_hook:env -> ident -> lident -> unit)
   : dsenv_hooks
 
-type withenv 'a = env -> 'a & env
-
-type foundname =
-  | Term_name of typ & list attribute
-  | Eff_name  of sigelt & lident
-
-val fail_or:  env -> (lident -> option 'a) -> lident -> 'a
-val fail_or2: env -> (ident -> option 'a) -> ident -> 'a
-
-val opens_and_abbrevs :env -> list (either open_module_or_namespace module_abbrev)
-val dep_graph: env -> FStarC.Parser.Dep.deps
-val set_dep_graph: env -> FStarC.Parser.Dep.deps -> env
-val ds_hooks : env -> dsenv_hooks
-val set_ds_hooks: env -> dsenv_hooks -> env
-val syntax_only: env -> bool
-val set_syntax_only: env -> bool -> env
-val qualify: env -> ident -> lident
 val set_iface: env -> bool -> env
 val iface: env -> bool
 val set_admitted_iface: env -> bool -> env
 val admitted_iface: env -> bool
-val expect_typ: env -> bool
 val set_expect_typ: env -> bool -> env
-val empty_env: FStarC.Parser.Dep.deps -> env
-val current_module: env -> lident
+val expect_typ: env -> bool
+val transitive_exported_ids: env -> lident -> ML (list string)
+val opens_and_abbrevs :env -> ML (list (either open_module_or_namespace module_abbrev))
+val open_modules: env -> list (lident & modul)
+val open_modules_and_namespaces: env -> ML (list lident)
+val module_abbrevs: env -> ML (list (ident & lident))
 val set_current_module: env -> lident -> env
 val clear_scope_mods: env -> env
-val open_modules: env -> list (lident & modul)
-val open_modules_and_namespaces: env -> list lident
-val module_abbrevs: env -> list (ident & lident)
-val iface_decls : env -> lident -> option (list Parser.AST.decl)
+val current_module: env -> ML lident
+val iface_decls : env -> lident -> ML (option (list Parser.AST.decl))
 val set_iface_decls: env -> lident -> list Parser.AST.decl -> env
 val iface_interleaving_init: env -> bool
-val try_lookup_id: env -> ident -> option term
-val shorten_module_path: env -> list ident -> bool -> (list ident & list ident)
-val shorten_lid: env -> lid -> lid
-val try_lookup_lid: env -> lident -> option term
-val try_lookup_lid_with_attributes: env -> lident -> option (term & list attribute)
-val try_lookup_lid_with_attributes_no_resolve: env -> lident -> option (term & list attribute)
-val try_lookup_lid_no_resolve: env -> lident -> option term
-val try_lookup_effect_name: env -> lident -> option lident
-val try_lookup_effect_name_and_attributes: env -> lident -> option (lident & list cflag)
-val try_lookup_effect_defn: env -> lident -> option eff_decl
+val qualify: env -> ident -> ML lident
+val syntax_only: env -> bool
+val set_syntax_only: env -> bool -> env
+val ds_hooks : env -> dsenv_hooks
+val set_ds_hooks: env -> dsenv_hooks -> env
+val empty_env: FStarC.Parser.Dep.deps -> ML env
+val dep_graph: env -> FStarC.Parser.Dep.deps
+val set_dep_graph: env -> FStarC.Parser.Dep.deps -> env
+val try_lookup_id: env -> ident -> ML (option term)
+val resolve_module_name: env:env -> lid:lident -> honor_ns:bool -> ML (option lident)
+val shorten_module_path: env -> list ident -> bool -> ML (list ident & list ident)
+val fv_qual_of_se : sigelt -> ML (option fv_qual)
+val try_lookup_effect_name: env -> lident -> ML (option lident)
+val try_lookup_effect_name_and_attributes: env -> lident -> ML (option (lident & list cflag))
+val try_lookup_effect_defn: env -> lident -> ML (option eff_decl)
+val is_effect_name: env -> lident -> ML bool
 (* [try_lookup_root_effect_name] is the same as
 [try_lookup_effect_name], but also traverses effect abbrevs. TODO:
 once indexed effects are in, also track how indices and other
 arguments are instantiated. *)
-val try_lookup_root_effect_name: env -> lident -> option lident
-val try_lookup_datacon: env -> lident -> option (fv & sigelt)
-val try_lookup_record_by_field_name: env -> lident -> option record_or_dc
+val try_lookup_root_effect_name: env -> lident -> ML (option lident)
+val lookup_letbinding_quals_and_attrs: env -> lident -> ML (list qualifier & list attribute)
+val try_lookup_definition: env -> lident -> ML (option term)
+(* private *) val try_lookup_lid': bool -> bool -> env -> lident -> ML (option (term & list attribute))
+val try_lookup_lid_with_attributes: env -> lident -> ML (option (term & list attribute))
+val try_lookup_lid: env -> lident -> ML (option term)
+val resolve_to_fully_qualified_name : env:env -> l:lident -> ML (option lident)
+val shorten_lid: env -> lid -> ML lid
+val try_lookup_lid_with_attributes_no_resolve: env -> lident -> ML (option (term & list attribute))
+val try_lookup_lid_no_resolve: env -> lident -> ML (option term)
+val try_lookup_datacon: env -> lident -> ML (option (fv & sigelt))
+val find_all_datacons: env -> lident -> ML (option (list lident))
+val try_lookup_record_by_field_name: env -> lident -> ML (option record_or_dc)
 (* [try_lookup_record_by_field_name_many] finds a record type that includes all of the given fields *)
-val try_lookup_record_by_field_name_many: env -> list lident -> option record_or_dc
-val try_lookup_record_type: env -> lident -> option record_or_dc
-val belongs_to_record: env -> lident -> record_or_dc -> bool
-val try_lookup_dc_by_field_name: env -> lident -> option (lident & bool)
-val try_lookup_definition: env -> lident -> option term
-val is_effect_name: env -> lident -> bool
-val find_all_datacons: env -> lident -> option (list lident)
-val lookup_letbinding_quals_and_attrs: env -> lident -> list qualifier & list attribute
-val resolve_module_name: env:env -> lid:lident -> honor_ns:bool -> option lident
-val resolve_to_fully_qualified_name : env:env -> l:lident -> option lident
-val fv_qual_of_se : sigelt -> option fv_qual
-
-val push_bv': env -> ident -> env & bv & used_marker
-val push_bv: env -> ident -> env & bv
-val push_top_level_rec_binding: env -> ident -> env & ref bool
-val push_sigelt: env -> sigelt -> env
-val push_namespace: env -> lident -> restriction -> env
-val push_include: env -> lident -> restriction -> env
-val push_module_abbrev : env -> ident -> lident -> env
-val resolve_name: env -> lident -> option (either bv fv)
-
+val try_lookup_record_by_field_name_many: env -> list lident -> ML (option record_or_dc)
+val try_lookup_record_type: env -> lident -> ML (option record_or_dc)
+val belongs_to_record: env -> lident -> record_or_dc -> ML bool
+val try_lookup_dc_by_field_name: env -> lident -> ML (option (lident & bool))
+(* private *) val unique:  bool -> bool -> env -> lident -> ML bool
+val push_bv': env -> ident -> ML (env & bv & used_marker)
+val push_bv: env -> ident -> ML (env & bv)
+val push_top_level_rec_binding: env -> ident -> ML (env & ref bool)
+val push_sigelt: env -> sigelt -> ML env
 (* Won't fail on duplicates, use with caution *)
-val push_sigelt_force : env -> sigelt -> env
-
-val pop: unit -> env
-val push: env -> env
-val rollback: option int -> env
-val snapshot: env -> (int & env)
-
-val finish_module_or_interface: env -> modul -> (env & modul)
-val enter_monad_scope: env -> ident -> env
-val export_interface: lident ->  env -> env
-
-val transitive_exported_ids: env -> lident -> list string
+val push_sigelt_force : env -> sigelt -> ML env
+val push_namespace: env -> lident -> restriction -> ML env
+val push_include: env -> lident -> restriction -> ML env
+val push_module_abbrev : env -> ident -> lident -> ML env
+(* private *) val check_admits: env -> modul -> ML modul
+(* private *) val finish:  env -> modul -> ML env
+val push: env -> ML env
+val pop: unit -> ML env
+val snapshot: env -> ML (int & env)
+val rollback: option int -> ML env
+val export_interface: lident ->  env -> ML env
+val finish_module_or_interface: env -> modul -> ML (env & modul)
 val module_inclusion_info : Type0
-val default_mii : module_inclusion_info
-val inclusion_info: env -> lident -> module_inclusion_info
-val prepare_module_or_interface: no_prelude:bool -> is_interface:bool -> is_admitted:bool -> env -> lident -> module_inclusion_info -> env & bool //pop the context when done desugaring
 instance val showable_mii: showable module_inclusion_info
-(* private *) val try_lookup_lid': bool -> bool -> env -> lident -> option (term & list attribute)
-(* private *) val unique:  bool -> bool -> env -> lident -> bool
-(* private *) val check_admits: env -> modul -> modul
-(* private *) val finish:  env -> modul -> env
-
+val default_mii : module_inclusion_info
+val inclusion_info: env -> lident -> ML module_inclusion_info
+val prepare_module_or_interface: no_prelude:bool -> is_interface:bool -> is_admitted:bool -> env -> lident -> module_inclusion_info -> ML (env & bool) //pop the context when done desugaring
+val enter_monad_scope: env -> ident -> ML env
+val fail_or:  env -> (lident -> option 'a) -> lident -> ML 'a
+val fail_or2: env -> (ident -> option 'a) -> ident -> ML 'a
+val resolve_name: env -> lident -> ML (option (either bv fv))
 val set_no_prelude : env -> bool -> env
